Challenge/Ripemd160/Submission/Proofs/Bytecode/J2Payload.lean
@@ -44,7 +44,7 @@ private def codePrefix : ByteArray :=
  ++   submissionByteChunk17
  ++   submissionByteChunk18
  ++   submissionByteChunk19
-private theorem codePrefix_size : codePrefix.size = 4625 := by
+private theorem codePrefix_size : codePrefix.size = 4626 := by
   simp only [codePrefix, ByteArray.size_append,
     submissionByteChunk0_size,
     submissionByteChunk1_size,
@@ -70,13 +70,13 @@ private theorem code_split : submissionBytecode = codePrefix ++ submissionByteCh
 
 private theorem tableRead (n : Nat) :
     MachineState.readPadded submissionBytecode (4938 + 20*((2337668504/n)%16)) 20 =
-      MachineState.readPadded submissionByteChunk20 (313 + 20*((2337668504/n)%16)) 20 := by
+      MachineState.readPadded submissionByteChunk20 (312 + 20*((2337668504/n)%16)) 20 := by
   rw [code_split, readPadded_append_right _ _ _ _ (by rw [codePrefix_size]; omega), codePrefix_size]
   congr 1
   omega
 
 private theorem tablePayload (n : Nat) (hn : Allowed n) :
-    MachineState.readPadded submissionByteChunk20 (313 + 20*((2337668504/n)%16)) 20 =
+    MachineState.readPadded submissionByteChunk20 (312 + 20*((2337668504/n)%16)) 20 =
       MachineState.readPadded payload (20*((2337668504/n)%16)) 20 := by
   rcases hn with rfl | rfl | rfl | rfl | rfl | rfl | rfl | rfl | rfl | rfl | rfl | rfl | rfl | rfl
   all_goals decide
